theories/SAst.v
@@ -30,6 +30,7 @@ Inductive sterm : Type :=
 | sCongEq (pA pu pv : sterm)
 | sCongRefl (pA pu : sterm)
 | sEqToHeq (p : sterm)
+| sHeqTypeEq (p : sterm)
 (* Packing *)
 | sPack (A1 A2 : sterm)
 | sProjT1 (p : sterm)
